# Saved by TopBraid on Tue Aug 30 11:14:01 PDT 2011
# baseURI: http://www.linkedmodel.org/1.2/schema/vaem-xina
# imports: http://www.linkedmodel.org/1.2/schema/vaem

@prefix dc:      <http://purl.org/dc/elements/1.1/> .
@prefix owl:     <http://www.w3.org/2002/07/owl#> .
@prefix rdf:     <http://www.w3.org/1999/02/22-rdf-syntax-ns#> .
@prefix rdfs:    <http://www.w3.org/2000/01/rdf-schema#> .
@prefix vaem:    <http://www.linkedmodel.org/schema/vaem#> .
@prefix vaem-xina:  <http://www.linkedmodel.org/1.2/schema/vaem-xina#> .
@prefix voag:    <http://voag.linkedmodel.org/schema/voag#> .
@prefix xsd:     <http://www.w3.org/2001/XMLSchema#> .

voag:VAEM-XINA-CatalogEntry
      rdf:type vaem:CatalogEntry ;
      rdfs:label "VAEM-XINA Catalog entry"^^xsd:string .

<http://www.linkedmodel.org/1.2/schema/vaem-xina>
      rdf:type owl:Ontology ;
      dc:author "Ralph Hodgson"^^xsd:string ;
      dc:subject "Names and Identifiers"^^xsd:string ;
      dc:title "Vocabulary for Attaching Essential Metadata for Names and Identifiers"^^xsd:string ;
      vaem:dateCreated "2011-08-01"^^vaem:dateUnion ;
      vaem:description "VAEM-XINA is an extension to VAEM to provide a vocabulary for  'Identifiers', 'Names', 'Acronyms' and 'Abbreviations'."^^xsd:string ;
      vaem:hasCatalogEntry
              voag:VAEM-XINA-CatalogEntry ;
      vaem:hasGraphRole vaem:SchemaGraph ;
      vaem:hasLicenseType voag:CC-SHAREALIKE_3PT0-US ;
      vaem:name "VAEM-XINA"^^xsd:string ;
      vaem:revision "1.2"^^xsd:string ;
      vaem:usesNonImportedResource
              dc:description , dc:title , dc:contributor , dc:subject , dc:author ;
      vaem:withAttributionTo
              voag:TopQuadrantAttribution ;
      owl:imports <http://www.linkedmodel.org/1.2/schema/vaem> ;
      owl:versionIRI <http://www.linkedmodel.org/1.2/schema/vaem-xina> ;
      owl:versionInfo "Created with TopBraid Composer"^^xsd:string .

vaem:abbreviation
      rdf:type owl:DatatypeProperty ;
      rdfs:comment "The property 'vaem:abbreviation' provides a common way to define a commonly used abbreviation on a resource."^^xsd:string ;
      rdfs:label "abbreviation"^^xsd:string .

vaem:acronym
      rdf:type owl:DatatypeProperty ;
      rdfs:comment "The property 'vaem:acronym' provides a common way to define a commonly used abbreviation on a resource."^^xsd:string ;
      rdfs:label "acronym"^^xsd:string .

vaem:hasIdentifier
      rdf:type owl:ObjectProperty ;
      rdfs:comment "The property 'vaemhasIdentifier' is intended for general use as a means to specifiy a unique reference to something. This is an object property that is a sub-property of 'vame:id'."^^xsd:string ;
      rdfs:label "has identifier"^^xsd:string ;
      rdfs:subPropertyOf vaem:id .

vaem:id
      rdf:type rdf:Property ;
      rdfs:comment "The property 'vaem:id' is intended for general use as a means to specifiy an identifier. The type of this property is intentionally set to 'rdf:Property' so that use of the property can allow both object and scaler values.  For this reason, the property is rangeless."^^xsd:string ;
      rdfs:label "id"^^xsd:string .

vaem:idString
      rdf:type owl:DatatypeProperty ;
      rdfs:comment "The property 'vaem:idString' is intended for general use as a means to specifiy a unique reference to something. This is a data property with a string range and is a sub-property of 'vame:id'."^^xsd:string ;
      rdfs:label "identifier"^^xsd:string ;
      rdfs:range xsd:string ;
      rdfs:subPropertyOf vaem:id .
