# baseURI: http://siemens.com/schemas/san
# imports: http://fonm.org/1.0/schema/core
# imports: http://www.w3.org/ns/ssn/systems/
# prefix: san

@prefix dc: <http://purl.org/dc/elements/1.1/> .
@prefix ext: <http://purl.obolibrary.org/obo/uberon/ext.owl#> .
@prefix fonm: <http://fonm.org/schema/fonm#> .
@prefix owl: <http://www.w3.org/2002/07/owl#> .
@prefix qudt: <http://qudt.org/schema/qudt#> .
@prefix rdf: <http://www.w3.org/1999/02/22-rdf-syntax-ns#> .
@prefix rdfs: <http://www.w3.org/2000/01/rdf-schema#> .
@prefix san: <http://siemens.com/schemas/san#> .
@prefix sh: <http://www.w3.org/ns/shacl#> .
@prefix skos: <http://www.w3.org/2004/02/skos/core#> .
@prefix sosa: <http://www.w3.org/ns/sosa/> .
@prefix ssn: <http://www.w3.org/ns/ssn/> .
@prefix unit: <http://qudt.org/vocab/unit#> .
@prefix vaem: <http://www.linkedmodel.org/schema/vaem#> .
@prefix xhtm: <http://www.w3.org/1999/xhtml> .
@prefix xsd: <http://www.w3.org/2001/XMLSchema#> .

<http://siemens.com/schemas/san>
  rdf:type owl:Ontology ;
  dc:contributor "Jack Hodges" ;
  dc:creator "Jack Hodges" ;
  dc:description "Semantic Actuator Framework" ;
  dc:subject "SAN" ;
  dc:title "The Siemens Semantic Actuator Framework Ontology" ;
  vaem:hasGraphRole vaem:SchemaGraph ;
  vaem:intent "The SAN is an actuation ontology that extends the SSN ontology to actuation."^^xsd:string ;
  vaem:namespace "http://siemens.com/schemas/san#"^^xsd:string ;
  vaem:namespacePrefix "san"^^xsd:string ;
  vaem:url "http://siemens.com/schemas/san"^^xsd:anyURI ;
  rdfs:label "SAN ontology"^^xsd:string ;
  owl:versionInfo "$Id: SCHEMA_san-v1.0.ttl 1954 2018-08-22 13:35:02Z jhodges $"^^xsd:string ;
  owl:imports <http://fonm.org/1.0/schema/core> ;
  owl:imports <http://www.w3.org/ns/ssn/systems/> ;
  owl:versionInfo "Created with TopBraid Composer" ;
.
san:ActuatingDevice
  rdf:type owl:Class ;
  rdfs:comment "Any device that can control a mechanism through actuation. As simple as a switch and as complex as a controller. Some affect single properties while others may control many properties." ;
  rdfs:label "Actuating device" ;
  rdfs:seeAlso "https://en.wikipedia.org/wiki/Actuator" ;
  rdfs:subClassOf fonm:Device ;
  rdfs:subClassOf san:Actuator ;
.
san:Actuation
  rdf:type owl:Class ;
  rdfs:comment "Actuation is a process that results in the control of a device, which controls the value of a phenomenon." ;
  rdfs:label "Actuation" ;
  rdfs:subClassOf sosa:Actuation ;
.
san:ActuationCapability
  rdf:type owl:Class ;
  rdfs:comment """Collects together actuation properties (accuracy, range, precision, etc) and the environmental conditions in which those properties hold, representing a specification of an actuator's capability in those conditions.

The conditions specified here are those that affect the actuation properties, while those in OperatingRange represent the actuator's standard operating conditions, including conditions that don't affect the observations.""" ;
  rdfs:label "Actuation Capability" ;
  rdfs:subClassOf ssn:Property ;
  rdfs:subClassOf [
      rdf:type owl:Restriction ;
      owl:allValuesFrom san:ActuationProperty ;
      owl:onProperty san:hasActuationProperty ;
    ] ;
  rdfs:subClassOf [
      rdf:type owl:Restriction ;
      owl:allValuesFrom ssn:Condition ;
      owl:onProperty ssn:inCondition ;
    ] ;
  rdfs:subClassOf [
      rdf:type owl:Restriction ;
      owl:allValuesFrom ssn:Property ;
      owl:onProperty ssn:forProperty ;
    ] ;
  rdfs:subClassOf [
      rdf:type owl:Restriction ;
      owl:minCardinality "0"^^xsd:nonNegativeInteger ;
      owl:onProperty san:hasActuationProperty ;
    ] ;
.
san:ActuationProperty
  rdf:type owl:Class ;
  rdfs:comment "An identifiable and observable characteristic of an actuator's actions or ability to invoke actions." ;
  rdfs:label "Actuation  Property" ;
  rdfs:subClassOf ssn:Property ;
.
san:ActuationValue
  rdf:type owl:Class ;
  rdfs:label "Actuation Value" ;
  rdfs:subClassOf ssn:Property ;
.
san:Actuator
  rdf:type owl:Class ;
  rdfs:comment "An actuator can do (implements) actuation: that is, an actuator is any entity that can follow an actuation/control method and thus control a device that produces some Property of a FeatureOfInterest.  Actuators may be physical devices, computational methods, a laboratory setup with a person following a method, or any other thing that can follow an Actuation Method to control a Property. Actuators require a source of energy and a control signal." ;
  rdfs:label "Actuator" ;
  rdfs:seeAlso "https://en.wikipedia.org/wiki/Actuator" ;
  rdfs:subClassOf fonm:Device ;
  rdfs:subClassOf sosa:Actuator ;
  rdfs:subClassOf [
      rdf:type owl:Restriction ;
      owl:allValuesFrom san:ActuationCapability ;
      owl:onProperty san:hasActuationCapability ;
    ] ;
  rdfs:subClassOf [
      rdf:type owl:Restriction ;
      owl:allValuesFrom ssn:Property ;
      owl:onProperty ssn:observes ;
    ] ;
  rdfs:subClassOf [
      rdf:type owl:Restriction ;
      owl:allValuesFrom ssn:Stimulus ;
      owl:onProperty ssn:detects ;
    ] ;
  rdfs:subClassOf [
      rdf:type owl:Restriction ;
      owl:cardinality "1"^^xsd:nonNegativeInteger ;
      owl:onProperty san:hasActuationValue ;
    ] ;
  rdfs:subClassOf [
      rdf:type owl:Restriction ;
      owl:cardinality "1"^^xsd:nonNegativeInteger ;
      owl:onProperty san:hasOperation ;
    ] ;
  rdfs:subClassOf [
      rdf:type owl:Restriction ;
      owl:onProperty ssn:implements ;
      owl:someValuesFrom san:Actuation ;
    ] ;
.
san:Operation
  rdf:type owl:Class ;
  rdfs:label "Operation" ;
  rdfs:subClassOf <http://www.ontologydesignpatterns.org/ont/dul/DUL.owl#Method> ;
.
san:hasActuationCapability
  rdf:type owl:ObjectProperty ;
  rdfs:comment "Relation from an Actuator to an ActuationCapability describing the actuation properties of the actuator." ;
  rdfs:label "has actuation capability" ;
  rdfs:subPropertyOf san:hasProperty ;
.
san:hasActuationProperty
  rdf:type owl:ObjectProperty ;
  rdfs:comment "Relation from an ActuationCapability to an ActuationProperty.  For example, to an accuracy (see notes at ssn:MeasurementCapability)." ;
  rdfs:label "has actuation property" ;
  rdfs:subPropertyOf san:hasProperty ;
.
san:hasActuationValue
  rdf:type rdf:Property ;
  rdfs:label "has actuation value" ;
  rdfs:range san:ActuationValue ;
.
san:hasOperation
  rdf:type rdf:Property ;
  rdfs:label "has operation" ;
  rdfs:range san:Operation ;
.
san:hasProperty
  rdf:type owl:ObjectProperty ;
  rdfs:label "has property" ;
  rdfs:subPropertyOf <http://www.loa-cnr.it/ontologies/DUL.owl#hasQuality> ;
.
